grounding lifting

Superposition_Calculus/Abstract_Substitution/Variable_Substitution.thy
@@ -2,6 +2,22 @@ theory Variable_Substitution
   imports Abstract_Substitution "HOL-Library.FSet" "HOL-Library.Multiset"
 begin
 
+locale finite_set =
+  fixes set :: "'b \<Rightarrow> 'a set"
+  assumes finite_set [simp]: "\<And>b. finite (set b)"
+begin
+
+abbreviation finite_set :: "'b \<Rightarrow> 'a fset" where 
+  "finite_set b \<equiv> Abs_fset (set b)"
+
+lemma finite_set': "set b \<in> {A. finite A}"
+  by simp
+
+lemma fset_finite_set [simp]: "fset (finite_set b) = set b"
+  using Abs_fset_inverse[OF finite_set'].
+
+end
+
 locale variable_substitution = 
   basic_substitution _ _ subst "\<lambda>a. vars a = {}" 
 for
@@ -54,9 +70,15 @@ lemma
 
 end*)
 
-locale finite_variables =
-  fixes vars :: "'expression \<Rightarrow> 'variable set"
-  assumes finite_vars [simp]: "\<And>a. finite (vars a)"
+locale finite_variables = finite_set vars for vars :: "'expression \<Rightarrow> 'variable set"
+begin
+
+lemmas finite_vars = finite_set finite_set'
+lemmas fset_finite_vars = fset_finite_set
+
+abbreviation "finite_vars \<equiv> finite_set"
+
+end
 
 locale all_subst_ident_iff_ground =
   fixes is_ground :: "'expression \<Rightarrow> bool" and subst 
@@ -71,11 +93,14 @@ locale grounding = variable_substitution
   assumes 
     range_from_ground_iff_is_ground: "{f. is_ground f} = range from_ground" and
     from_ground_inverse: "\<And>g. to_ground (from_ground g) = g"
-    (*surj_to_ground: "surj to_ground" and inj_from_ground: "inj from_ground"*)
 begin
 
 definition groundings ::"'a \<Rightarrow> 'g set" where
   "groundings a = { to_ground (a \<cdot> \<gamma>) | \<gamma>. is_ground (a \<cdot> \<gamma>) }"
+
+lemma to_ground_from_ground_id: "to_ground \<circ> from_ground = id"
+  using from_ground_inverse
+  by auto
 
 lemma surj_to_ground: "surj to_ground"
   using from_ground_inverse
@@ -98,22 +123,26 @@ lemma ground_is_ground: "is_ground (from_ground g)"
   using range_from_ground_iff_is_ground
   by blast
 
+lemma is_ground_iff_range_from_ground: "is_ground f \<longleftrightarrow> f \<in> range from_ground"
+  using range_from_ground_iff_is_ground
+  by auto
+
 lemma to_ground_inverse: 
   assumes "is_ground f"
   shows "from_ground (to_ground f) = f"
-  using assms 
-  by (metis (mono_tags, lifting) from_ground_inverse inj_on_eq_iff inj_on_to_ground mem_Collect_eq 
-        rangeI range_from_ground_iff_is_ground)
+  using inj_on_to_ground from_ground_inverse is_ground_iff_range_from_ground assms
+  unfolding inj_on_def
+  by blast
 
 end
 
-(* TODO: base_variable_substitution *)
-locale variable_substitution_base = variable_substitution 
+locale base_variable_substitution = variable_substitution 
   where subst = subst
   for subst :: "'expression \<Rightarrow> ('variable \<Rightarrow> 'expression) \<Rightarrow> 'expression"  (infixl "\<cdot>" 70) +
-  assumes 
-    is_ground_iff: "\<And>exp. is_ground (exp \<cdot> \<gamma>) \<longleftrightarrow> (\<forall>x \<in> vars exp. is_ground (\<gamma> x))" and
-   ground_exists: "\<exists>exp. is_ground exp"
+  assumes
+    is_grounding_iff_vars_grounded: 
+      "\<And>exp. is_ground (exp \<cdot> \<gamma>) \<longleftrightarrow> (\<forall>x \<in> vars exp. is_ground (\<gamma> x))" and
+    ground_exists: "\<exists>exp. is_ground exp"
 begin 
 
 lemma obtain_ground_subst:
@@ -124,7 +153,7 @@ proof-
     using ground_exists by blast
 
   then have "is_ground_subst  (\<lambda>_. g)"
-    by (simp add: is_ground_iff is_ground_subst_def)
+    by (simp add: is_grounding_iff_vars_grounded is_ground_subst_def)
 
   then show ?thesis
     using that
@@ -145,7 +174,7 @@ proof-
     \<gamma>':  "\<gamma>' = (\<lambda>var. if var \<in> vars exp then \<gamma> var else \<gamma>'' var)"
 
   have "is_ground_subst \<gamma>'"
-    using assms \<gamma>'' is_ground_iff
+    using assms \<gamma>'' is_grounding_iff_vars_grounded
     unfolding \<gamma>' is_ground_subst_def
     by simp
 
@@ -161,32 +190,25 @@ qed
 lemma ground_subst_upd [simp]:
   assumes "is_ground update" "is_ground (exp \<cdot> \<gamma>)" 
   shows "is_ground (exp \<cdot> \<gamma>(var := update))"
-  using assms is_ground_iff by auto
+  using assms is_grounding_iff_vars_grounded by auto
 
 end
-  
 
-(* TODO: based_variable_substitution? *)
-locale variable_substitution_expansion = base: variable_substitution_base + 
-  variable_substitution where
-  subst = expanded_subst and 
-  id_subst = "id_subst" and 
-  comp_subst = comp_subst and 
-  vars = expanded_vars 
-for expanded_subst expanded_vars +
+locale based_variable_substitution = 
+  base: base_variable_substitution where subst = base_subst and vars = base_vars + 
+  variable_substitution
+for base_subst base_vars +
 assumes
-  expanded_vars_vars: 
-    "(\<forall>x. is_ground (expanded_subst x \<gamma>)) \<longleftrightarrow> (\<forall>x. base.is_ground (x \<cdot> \<gamma>))" and
-  is_ground_iff:
-  "is_ground (expanded_subst exp \<gamma>) \<longleftrightarrow> (\<forall>x \<in> expanded_vars exp. base.is_ground (\<gamma> x))"
+  ground_subst_base_ground_subst: 
+    "(\<forall>exp. is_ground (exp \<cdot> \<gamma>)) \<longleftrightarrow> (\<forall>base_exp. base.is_ground (base_subst base_exp \<gamma>))" and
+  is_grounding_iff_vars_grounded: 
+    "\<And>exp. is_ground (exp \<cdot> \<gamma>) \<longleftrightarrow> (\<forall>x \<in> vars exp. base.is_ground (\<gamma> x))"
 begin
 
-(* TODO: name *)
-lemma is_ground_subst_iff_base_is_ground_subst [simp]: 
+lemma is_ground_subst_iff_base [simp]: 
   "is_ground_subst \<gamma> \<longleftrightarrow> base.is_ground_subst \<gamma>"
-  unfolding is_ground_subst_def  base.is_ground_subst_def
-  using expanded_vars_vars
-  by presburger
+  unfolding is_ground_subst_def base.is_ground_subst_def
+  using ground_subst_base_ground_subst.
 
 lemma obtain_ground_subst:
   obtains \<gamma> 
@@ -194,49 +216,45 @@ lemma obtain_ground_subst:
   using base.obtain_ground_subst by auto
 
 lemma ground_subst_extension:
-  assumes "is_ground (expanded_subst exp \<gamma>)"
+  assumes "is_ground (exp \<cdot> \<gamma>)"
   obtains \<gamma>'
-  where "expanded_subst exp \<gamma> = expanded_subst exp \<gamma>'" and "is_ground_subst \<gamma>'"
-  by (metis all_subst_ident_if_ground assms is_ground_subst_comp_right obtain_ground_subst 
-       subst_comp_subst)
+  where "exp \<cdot> \<gamma> = exp \<cdot> \<gamma>'" and "is_ground_subst \<gamma>'"
+  using obtain_ground_subst assms
+  by (metis all_subst_ident_if_ground is_ground_subst_comp_right subst_comp_subst)
 
 lemma ground_subst_upd [simp]:
-  assumes "base.is_ground update" "is_ground (expanded_subst exp \<gamma>)" 
-  shows "is_ground (expanded_subst exp (\<gamma>(var := update)))"
-  using base.ground_subst_upd assms is_ground_iff by simp  
+  assumes "base.is_ground update" "is_ground (exp \<cdot> \<gamma>)" 
+  shows "is_ground (exp \<cdot> \<gamma>(var := update))"
+  using base.ground_subst_upd assms is_grounding_iff_vars_grounded by simp  
 
 lemma ground_exists: "\<exists>exp. is_ground exp"
   using base.ground_exists
-  by (meson is_ground_iff)
+  by (meson is_grounding_iff_vars_grounded)
 
 end
 
-(* TODO: Names *)
 locale variable_substitution_lifting = 
-  lifted: variable_substitution 
-  where comp_subst = comp_subst and id_subst = id_subst and subst = base_subst and 
-    vars = base_vars
-  for 
-    id_subst :: "'variable \<Rightarrow> 'base_expression" and
-    base_vars :: "'sub_expression \<Rightarrow> 'variable set" and
-    comp_subst base_subst +
-  fixes 
+  sub: variable_substitution 
+  where subst = sub_subst and vars = sub_vars
+  for
+    sub_vars :: "'sub_expression \<Rightarrow> 'variable set" and
+    sub_subst :: "'sub_expression \<Rightarrow> ('variable \<Rightarrow> 'base_expression) \<Rightarrow> 'sub_expression" +
+  fixes
     map :: "('sub_expression \<Rightarrow> 'sub_expression) \<Rightarrow> 'expression \<Rightarrow> 'expression" and
     to_set :: "'expression \<Rightarrow> 'sub_expression set"
   assumes 
     map_comp: "\<And>d f g. map f (map g d) = map (f \<circ> g) d" and
     map_id: "map id d = d" and
     map_cong: "\<And>d f g. (\<And>c. c \<in> to_set d \<Longrightarrow> f c = g c) \<Longrightarrow> map f d = map g d" and
-    (* TODO: name *)
-    Union_range_to_set: "\<And>c. \<exists>d. c \<in> to_set d" and
+    exists_expression: "\<And>c. \<exists>d. c \<in> to_set d" and
     to_set_map: "\<And>d f. to_set (map f d) = f ` to_set d" 
 begin
 
 definition vars :: "'expression \<Rightarrow> 'variable set" where
-  "vars d \<equiv> \<Union> (base_vars ` to_set d)"
+  "vars d \<equiv> \<Union> (sub_vars ` to_set d)"
 
 definition subst :: "'expression \<Rightarrow> ('variable \<Rightarrow> 'base_expression) \<Rightarrow> 'expression" where
-  "subst d \<sigma> \<equiv> map (\<lambda>c. base_subst c \<sigma>) d"
+  "subst d \<sigma> \<equiv> map (\<lambda>c. sub_subst c \<sigma>) d"
 
 lemma map_id_cong: 
   assumes "\<And>c. c \<in> to_set d \<Longrightarrow> f c = c"  
@@ -253,22 +271,21 @@ lemma to_set_map_not_ident:
 
 lemma subst_in_to_set_subst:
   assumes "c \<in> to_set d" 
-  shows "base_subst c \<sigma> \<in> to_set (subst d \<sigma>)"
+  shows "sub_subst c \<sigma> \<in> to_set (subst d \<sigma>)"
   unfolding subst_def
   using assms to_set_map by auto
 
 
-sublocale variable_substitution where
-  comp_subst = comp_subst and id_subst = id_subst and subst = subst and vars = vars
+sublocale variable_substitution where subst = subst and vars = vars
 proof unfold_locales
   show "\<And>x a b. subst x (comp_subst a b) = subst (subst x a) b"
-    using lifted.subst_comp_subst
+    using sub.subst_comp_subst
     unfolding subst_def map_comp comp_apply
     by presburger
 next
   show "\<And>x. subst x id_subst = x"
     using map_id
-    unfolding subst_def lifted.subst_id_subst id_def.
+    unfolding subst_def sub.subst_id_subst id_def.
 next
    show "\<And>x. vars x = {} \<Longrightarrow> \<forall>\<sigma>. subst x \<sigma> = x"
      unfolding vars_def subst_def    
@@ -277,22 +294,22 @@ next
 next
   show "\<And>a \<sigma> \<tau>. (\<And>x. x \<in> vars a \<Longrightarrow> \<sigma> x = \<tau> x) \<Longrightarrow> subst a \<sigma> = subst a \<tau> "
     unfolding vars_def subst_def
-    using map_cong lifted.subst_eq
+    using map_cong sub.subst_eq
     by (meson UN_I)
 qed
 
 (* TODO: name *)
 lemma is_ground_iff_base_is_ground: 
-  "(\<forall>d. is_ground (subst d \<gamma>)) \<longleftrightarrow> (\<forall>c. lifted.is_ground (base_subst c \<gamma>))"
-proof(rule iffI allI; rule allI)
+  "(\<forall>d. is_ground (subst d \<gamma>)) \<longleftrightarrow> (\<forall>c. sub.is_ground (sub_subst c \<gamma>))"
+proof(intro iffI allI)
   fix c 
   assume all_d_ground: "\<forall>d. is_ground (subst d \<gamma>)"
-  show "lifted.is_ground (base_subst c \<gamma>)"
+  show "sub.is_ground (sub_subst c \<gamma>)"
   proof(rule ccontr)
-    assume c_not_ground: "\<not>lifted.is_ground (base_subst c \<gamma>)"
+    assume c_not_ground: "\<not>sub.is_ground (sub_subst c \<gamma>)"
 
     then obtain d where "c \<in> to_set d"
-      using Union_range_to_set by auto
+      using exists_expression by auto
 
     then have "\<not>is_ground (subst d \<gamma>)"
       using c_not_ground to_set_map 
@@ -305,7 +322,7 @@ proof(rule iffI allI; rule allI)
   qed
 next
   fix d
-  assume all_c_ground: "\<forall>c. lifted.is_ground (base_subst c \<gamma>)"
+  assume all_c_ground: "\<forall>c. sub.is_ground (sub_subst c \<gamma>)"
 
   then show "is_ground (subst d \<gamma>)"
     unfolding vars_def subst_def
@@ -314,27 +331,35 @@ next
 qed
 
 lemma is_ground_subst_iff_base_is_ground_subst [simp]: 
-  "is_ground_subst \<gamma> \<longleftrightarrow> lifted.is_ground_subst \<gamma>"
-  unfolding is_ground_subst_def  lifted.is_ground_subst_def
+  "is_ground_subst \<gamma> \<longleftrightarrow> sub.is_ground_subst \<gamma>"
+  unfolding is_ground_subst_def sub.is_ground_subst_def
   using is_ground_iff_base_is_ground
   by presburger
+
+lemma to_set_is_ground:
+  assumes "sub \<in> to_set expr" "is_ground expr"
+  shows "sub.is_ground sub"
+  using assms
+  by (simp add: vars_def)
+
+lemma to_set_is_ground_subst:
+  assumes "sub \<in> to_set expr"  "is_ground (subst expr \<gamma>)"  
+  shows "sub.is_ground (sub_subst sub \<gamma>)"
+  using assms
+  by (meson subst_in_to_set_subst to_set_is_ground)
 
 end
 
 locale based_variable_substitution_lifting = 
-  variable_substitution_lifting where id_subst = id_subst and base_vars = base_vars and 
-  comp_subst = comp_subst and base_subst = base_subst and map = map and to_set = to_set +
-  base: variable_substitution_base
-  where comp_subst = comp_subst and id_subst = id_subst and subst = base'_subst and vars = base'_vars
-  for id_subst base_vars comp_subst base_subst map to_set base'_subst base'_vars +
-(* TODO: find way to not have provide this manually*)
-assumes lifted_is_ground_iff:
-  "\<And>exp \<gamma>. lifted.is_ground (base_subst exp \<gamma>) \<longleftrightarrow> (\<forall>x. x \<in> (base_vars exp) \<longrightarrow> base.is_ground (\<gamma> x))"
+  variable_substitution_lifting +
+  base: base_variable_substitution where subst = base_subst and vars = base_vars
+for base_subst base_vars +
+assumes sub_is_ground_iff: 
+  "\<And>exp \<gamma>. sub.is_ground (sub_subst exp \<gamma>) \<longleftrightarrow> (\<forall>x \<in> sub_vars exp. base.is_ground (\<gamma> x))"
 begin
 
-lemma is_ground_iff:
-  "is_ground (subst exp \<gamma>) \<longleftrightarrow> (\<forall>x. x \<in> (vars exp) \<longrightarrow> base.is_ground (\<gamma> x))"
-  using lifted_is_ground_iff subst_def to_set_map vars_def
+lemma is_ground_iff: "is_ground (subst exp \<gamma>) \<longleftrightarrow> (\<forall>x \<in> vars exp. base.is_ground (\<gamma> x))"
+  using sub_is_ground_iff subst_def to_set_map vars_def
   by auto
 
 lemma obtain_ground_subst:
@@ -363,24 +388,102 @@ end
 
 locale finite_variables_lifting = 
   variable_substitution_lifting + 
-  lifted: finite_variables where vars = base_vars +
-  assumes finite_to_set: "\<And>d. finite (to_set d)"
+  sub: finite_variables where vars = sub_vars +
+  to_set: finite_set where set = to_set
 begin
 
-sublocale finite_variables 
-  where vars = vars
-proof unfold_locales
-  show "\<And>a. finite (vars a)"
-    unfolding vars_def
-    by (simp add: finite_to_set)
-qed
+abbreviation to_fset :: "'d \<Rightarrow> 'c fset" where 
+  "to_fset \<equiv> to_set.finite_set"
+
+lemmas finite_to_set = to_set.finite_set to_set.finite_set'
+lemmas fset_to_fset = to_set.fset_finite_set
+
+sublocale finite_variables where vars = vars
+  by unfold_locales (simp add: vars_def)
 
 end
 
-(* TODO: base \<rightarrow> lifted *)
+locale grounding_lifting = 
+  variable_substitution_lifting where sub_vars = sub_vars and sub_subst = sub_subst and map = map + 
+  sub: grounding where vars = sub_vars and subst = sub_subst and to_ground = sub_to_ground and 
+  from_ground = sub_from_ground 
+for
+  sub_to_ground :: "'sub \<Rightarrow> 'ground_sub" and 
+  sub_from_ground :: "'ground_sub \<Rightarrow> 'sub" and
+  sub_vars :: "'sub \<Rightarrow> 'variable set" and 
+  sub_subst :: "'sub \<Rightarrow> ('variable \<Rightarrow> 'base) \<Rightarrow> 'sub" and
+  map :: "('sub \<Rightarrow> 'sub) \<Rightarrow> 'expr \<Rightarrow> 'expr" +
+fixes
+  to_ground_map :: "('sub \<Rightarrow> 'ground_sub) \<Rightarrow> 'expr \<Rightarrow> 'ground_expr" and
+  from_ground_map :: "('ground_sub \<Rightarrow> 'sub) \<Rightarrow> 'ground_expr \<Rightarrow> 'expr" and
+  ground_map :: "('ground_sub \<Rightarrow> 'ground_sub) \<Rightarrow> 'ground_expr \<Rightarrow> 'ground_expr" and
+  to_set_ground :: "'ground_expr \<Rightarrow> 'ground_sub set"
+assumes 
+  (* TODO: *)
+  (*to_ground_map_cong: "\<And>d f g. (\<And>c. c \<in> to_set d \<Longrightarrow> f c = g c) \<Longrightarrow> to_ground_map f d = to_ground_map g d" and
+  from_ground_map_cong: "\<And>d f g. (\<And>c. c \<in> to_set_ground d \<Longrightarrow> f c = g c) \<Longrightarrow> from_ground_map f d = from_ground_map g d" and*)
+  (*to_set_to_ground_map: "\<And>d f. to_set_ground (to_ground_map f d) = f ` to_set d" and*)
+  to_set_from_ground_map: "\<And>d f. to_set (from_ground_map f d) = f ` to_set_ground d" and
+  map_comp': "\<And>d f g. from_ground_map f (to_ground_map g d) = map (f \<circ> g) d" and
+  ground_map_comp: "\<And>d f g. to_ground_map f (from_ground_map g d) = ground_map (f \<circ> g) d" and
+  (*ground_map_cong: "\<And>d f g. (\<And>c. c \<in> to_set_ground d \<Longrightarrow> f c = g c) \<Longrightarrow> ground_map f d = ground_map g d" and*)
+  (*to_set_ground_map: "\<And>d f. to_ground_set (ground_map f d) = f ` to_ground_set d" and*)
+  ground_map_id: "ground_map id g = g"
+begin
+
+definition to_ground where "to_ground expr \<equiv> to_ground_map sub_to_ground expr"
+
+definition from_ground where "from_ground expr \<equiv> from_ground_map sub_from_ground expr"
+
+sublocale grounding where 
+  vars = vars and subst = subst and to_ground = to_ground and from_ground = from_ground
+proof unfold_locales
+  have "\<And>expr. vars expr = {} \<Longrightarrow> expr \<in> range from_ground"
+  proof-
+    fix expr
+    assume "vars expr = {}"
+    then have "\<forall>sub\<in>to_set expr. sub \<in> range sub_from_ground"
+      by (simp add: sub.is_ground_iff_range_from_ground vars_def)
+
+    then have "\<forall>sub\<in>to_set expr. (\<exists>sub_ground. sub_from_ground sub_ground = sub)"
+      by fast
+
+    then have "\<exists>ground_expr. from_ground ground_expr = expr"
+      unfolding from_ground_def
+      by (metis comp_eq_dest_lhs map_comp' map_id_cong)
+
+    then show "expr \<in> range from_ground"
+      unfolding from_ground_def
+      by blast
+  qed
+
+  moreover have "\<And>expr x. x \<in> vars (from_ground expr) \<Longrightarrow> False"
+  proof-
+    fix expr x
+    assume "x \<in> vars (from_ground expr)"
+    then show False
+      unfolding vars_def from_ground_def
+      using sub.ground_is_ground to_set_from_ground_map by auto
+  qed
+
+  ultimately show "{f. vars f = {}} = range from_ground"
+    by blast   
+next
+  show "\<And>g. to_ground (from_ground g) = g"
+    using ground_map_id
+    unfolding to_ground_def from_ground_def ground_map_comp sub.to_ground_from_ground_id.
+qed
+
+lemma "to_set (from_ground expr) = sub_from_ground ` (to_set_ground expr)"
+  unfolding from_ground_def
+  by (simp add: to_set_from_ground_map)
+
+end
+
+
 locale all_subst_ident_iff_ground_lifting = 
   finite_variables_lifting +  
-  lifted: all_subst_ident_iff_ground where subst = base_subst and is_ground = lifted.is_ground
+  sub: all_subst_ident_iff_ground where subst = sub_subst and is_ground = sub.is_ground
 begin
 
 sublocale all_subst_ident_iff_ground 
@@ -398,12 +501,12 @@ proof unfold_locales
     proof(rule ccontr)
       assume "\<not>is_ground d"
 
-      then obtain c where c_in_d: "c \<in> to_set d" and c_not_ground: "\<not>lifted.is_ground c"
+      then obtain c where c_in_d: "c \<in> to_set d" and c_not_ground: "\<not>sub.is_ground c"
         unfolding vars_def
         by blast
 
-      then obtain \<sigma> where "base_subst c \<sigma> \<noteq> c" and "base_subst c \<sigma> \<notin> to_set d"
-        using lifted.exists_non_ident_subst finite_to_set
+      then obtain \<sigma> where "sub_subst c \<sigma> \<noteq> c" and "sub_subst c \<sigma> \<notin> to_set d"
+        using sub.exists_non_ident_subst finite_to_set
         by blast
         
       then show False
@@ -419,13 +522,13 @@ next
   then have finite_cs: "finite (\<Union>(to_set ` insert d ds))"
     using finite_to_set by blast
 
-  obtain c where c_in_d: "c \<in> to_set d" and c_not_ground: "\<not>lifted.is_ground c"
+  obtain c where c_in_d: "c \<in> to_set d" and c_not_ground: "\<not>sub.is_ground c"
     using d_not_ground
     unfolding vars_def
     by blast
 
-  obtain \<sigma> where \<sigma>_not_ident: "base_subst c \<sigma> \<noteq> c" "base_subst c \<sigma> \<notin> \<Union> (to_set ` insert d ds)"
-    using lifted.exists_non_ident_subst[OF finite_cs c_not_ground]
+  obtain \<sigma> where \<sigma>_not_ident: "sub_subst c \<sigma> \<noteq> c" "sub_subst c \<sigma> \<notin> \<Union> (to_set ` insert d ds)"
+    using sub.exists_non_ident_subst[OF finite_cs c_not_ground]
     by blast
 
   then have "subst d \<sigma> \<noteq> d"
@@ -443,9 +546,5 @@ next
 qed
 
 end
-
-locale mylifting = 
-  based_variable_substitution_lifting + 
-  all_subst_ident_iff_ground_lifting 
 
 end
